# Special functions



{{< include ../math.qmd >}}


## Gamma functions

::: {#def-gamma-function}
## Gamma function
Let $z$ be any complex number that $\mathfrak R(z)>0$. Then 
$$
\Gamma(z)=\int_0^{\infty}t^{z-1}\me^{-t}\dl3t.
$$ {#eq-gamma-function}
:::


::: {#thm-gamma-factorial}
$$
\Gamma(z+1)=z\Gamma(z).
$$ {#eq-gamma-factorial}
::: 
::: {.proof}
$$
\begin{split}
    \Gamma(z+1)&=\int_0^{\infty}t^{z+1-1}\me^{-t}\dl3t=-\int_0^{\infty}t^{z+1-1}\dl3\me^{-t}\\
    &=-t\me^{-t}\biggr\rvert_0^{\infty}+\int_0^{\infty}\me^{-t}\dl3t^{z}=\int_0^{\infty}zt^{z-1}\me^{-t}\dl3t=z\Gamma(z).
\end{split}
$$

:::




## Beta functions


::: {#def-beta-function}
## Beta function
Let $z_1$, $z_2$ be two complex numbers that $\mathfrak R(z_1),\mathfrak R(z_2)>0$. Then
$$
B(z_1,z_2)=\int_0^1t^{z_1-1}(1-t)^{z_2-1}\dl3t.
$$ {#eq-beta-function}
:::


::: {#thm-beta-gammarelation}
## Relations between Beta functions and Gamma functions
$$
\Gamma(\alpha)\Gamma(\beta)=\Gamma(\alpha+\beta)B(\alpha, \beta).
$$ {#eq-beta-gammarelation}
:::

::: {.proof}
Use the following trick to change a product of two integrals into a double integral.
$$
\begin{align}
\Gamma(\alpha)\Gamma(\beta)&=\int_0^{\infty}u^{\alpha-1}\me^{-u}\dl3u\int_0^{\infty}v^{\beta-1}\me^{-v}\dl3v\\
&=\int_0^{\infty}\int_0^{\infty}u^{\alpha-1}v^{\beta-1}\me^{-u-v}\dl3u\dl3v.
\end{align}
$$

Set $u=st$, $v=s-st$. Then $s=u+v$, $t=\dfrac{u}{u+v}$, and $\abs{\dfrac{\partial(u,v)}{\partial(s,t)}}=\abs{\mqty[t&s\\1-t&-s]}=s$. Then
$$\begin{split}
    \Gamma(\alpha)\Gamma(\beta)&=\int_0^{\infty}\int_0^{\infty}u^{\alpha-1}v^{\beta-1}\me^{-u-v}\dl3u\dl3v\\
    &=\int_{v=0}^{v=\infty}\int_{u=0}^{u=\infty}(st)^{\alpha-1}(s(1-t))^{\beta-1}\me^{-s}s\dl3s\dl3t\\
    &=\int_{t=0}^{t=1}\int_{s=0}^{s=\infty}s^{\alpha+\beta-1}t^{\alpha-1}(1-t)^{\beta-1}\me^{-s}\dl3s\dl3t\\
    &=\int_{0}^{\infty}s^{\alpha+\beta-1}\me^{-s}\dl3s\int_{0}^{1}t^{\alpha-1}(1-t)^{\beta-1}\dl3t\\
    &=\Gamma(\alpha+\beta)B(\alpha,\beta).
\end{split}$$ 

:::

